Worked with Cezar yesterday to brainstorm how to make theta history independence proof go through.

rupicola/io/IO.fst
@@ -2,6 +2,7 @@ module IO
 
 (** we only have bools in STLC right now **)
 open Trace
+open STLC
 
 noeq
 type io (a:Type u#a) : Type u#a =
@@ -62,15 +63,130 @@ let lem_theta_write (b:bool) (x:io_res OWrite b) (h:history) (lt:local_trace h) 
         (ensures wp2p (theta (write b)) h lt x) =
   assert (theta (write b) == (fun (h:history) (p:hist_post h (resexn unit)) -> (forall (lt:local_trace h) (r:resexn unit). lt == [EvWrite b r] ==> p (lt @ []) r))) by (assert (lt @ []) == lt; FStar.Tactics.compute ())
 
+(*//requires lt == []
+//ensures wp2p (theta (return x))
+
+assume val get_lt (h h':history) (lt:local_trace h) : (lt':local_trace h') // indution on lt
+
+let hist_monotonic (wp:hist 'a) :
+Lemma (forall h h' (p':hist_post h' 'a). (wp h' p' ==> wp h (fun lt res -> p' (get_lt h h' lt) res))) = admit ()
+
+// equivalent up to renaming of local traces*)
+
+let rec theta_monotonic_hist (m:io 'a) :
+Lemma (forall h h' (p':hist_post h' 'a). (theta m h' p' ==> theta m h (fun lt res -> p' (get_lt h h' lt) res))) =
+  match m with
+  | Return x -> begin
+    introduce forall h h' p'. theta m h' p' ==> theta m h (fun lt res -> p' (get_lt h h' lt) res) with begin
+      introduce _ ==> _ with _. begin
+        let lt' : local_trace h' = [] in
+        let lt : local_trace h = [] in
+        assert (theta m h' p' == p' lt' x);
+        assert (theta m h (fun lt res -> p' (get_lt h h' lt) res) == (p' (get_lt h h' lt) x));
+        assume (p' lt' x ==> p' (get_lt h h' lt) x)
+        //assume (get_lt h h' lt == lt')
+        //admit ()
+      end
+    end
+    end
+  | Call o args k -> begin
+    introduce forall h h' p'. theta m h' p' ==> theta m h (fun lt res -> p' (get_lt h h' lt) res) with begin
+      introduce _ ==> _ with _. begin
+        assert (theta (Call o args k) == hist_bind (op_wp o args) (fun r -> theta (k r))) by (FStar.Tactics.compute ());
+        assert (hist_bind (op_wp o args) (fun r -> theta (k r)) h' p' == (op_wp o args) h' (hist_post_bind h' (fun r -> theta (k r)) p')) by (FStar.Tactics.compute ());
+        assert ((op_wp o args) h' (hist_post_bind h' (fun r -> theta (k r)) p') == forall r. theta (k r) (h'++[op_to_ev o args r]) (fun lt' r -> p' ([op_to_ev o args r] @ lt') r)) by (FStar.Tactics.compute ());
+        introduce forall r. theta (k r) (h++[op_to_ev o args r]) (fun lt' r -> (p' (get_lt h h' ([op_to_ev o args r] @ lt')) r with begin
+          theta_monotonic_hist (k r);
+        end
+        //assume (forall r. theta (k r) (h++[op_to_ev o args r]) (fun lt' r -> (p' (get_lt h h' ([op_to_ev o args r] @ lt')) r));
+        //assume ((op_wp o args) h (fun lt r -> theta (k r) (h++lt) (fun lt' r -> p' (get_lt h h' (lt @ lt')) r)))
+        //assert (theta m h (fun lt res -> p' (get_lt h h' lt) res) == (p' (get_lt h h' lt) x));
+        //assume (p' lt' x ==> p' (get_lt h h' lt) x)
+        //assume (get_lt h h' lt == lt')
+        admit ()
+      end
+    end
+    end
+
 let theta_history_independence #a (m:io a) (h h':history) (lt:local_trace h) (lt':local_trace h') (fs_r:a) :
   Lemma (requires wp2p (theta m) h lt fs_r /\ lt == lt')
-        (ensures wp2p (theta m) h' lt' fs_r) =
-  introduce forall p'. (theta m) h' p' ==> p' lt' fs_r with begin
+        (ensures wp2p (theta m) h' (get_lt h h' lt) fs_r) =
+  match m with
+  | Return x -> begin
+    assert (wp2p (theta m) h lt fs_r);
+    assert (forall p. (theta m) h p ==> p [] x);
+    introduce forall (p':hist_post h' a). (theta m) h' p' ==> p' lt' fs_r with begin
+      introduce (theta m) h' p' ==> p' lt' fs_r with _. begin
+      
+        let p : hist_post h a = fun lt res -> p' (get_lt h h' lt) res in
+        eliminate forall p. (theta m) h p ==> p lt fs_r with p;
+        assert ((theta m) h' p');
+        hist_wp_monotonic' (theta m);
+        assert (p lt fs_r);
+        assert (p' (get_lt h h' lt) fs_r);
+        assert ((get_lt h h' lt) == lt')
+  
+        //admit ()
+        //assert ((theta m) h p ==> p lt fs_r);
+        //admit ()
+      end
+    end
+    //assume (forall p'. (theta m) h' p' ==> p' [] x);
+    //assert (lt == []);
+    //assert (fs_r == x);
+    //assume (wp2p (theta m) h' [] x)
+    //admit ()
+    end
+  | Call o args k -> admit ()
+  (*introduce forall (p':hist_post h' a). (theta m) h' p' ==> p' lt' fs_r with begin
     introduce (theta m) h' p' ==> p' lt' fs_r with _. begin
-      let p : hist_post h a = fun _ _ -> p' lt fs_r in
+      
+      let p : hist_post h a = fun lt res -> p' (get_lt h h' lt) res in
       eliminate forall p. (theta m) h p ==> p lt fs_r with p;
       assert ((theta m) h' p');
-      assume ((theta m) h p)
+      assert ((theta m) h p ==> p lt fs_r);
+      admit ()
     end
-  end
+  end*)
+
+
+
+
+
+
+
+let theta_history_independence' #a (m:io a) (h h':history) (lt:local_trace h) (lt':local_trace h') (fs_r:a) :
+  Lemma (requires wp2p (theta m) h lt fs_r /\ lt == lt')
+        (ensures wp2p (theta m) h' lt' fs_r) =
+  match m with
+  | Return x -> begin
+    assert (wp2p (theta m) h lt fs_r);
+    assert (forall p. (theta m) h p ==> p [] x);
+    introduce forall (p':hist_post h' a). (theta m) h' p' ==> p' lt' fs_r with begin
+      introduce (theta m) h' p' ==> p' lt' fs_r with _. begin
+      
+        let p : hist_post h a = fun lt res -> p' (get_lt h h' lt) res in
+        eliminate forall p. (theta m) h p ==> p lt fs_r with p;
+        assert ((theta m) h' p');
+        assert ((theta m) h p ==> p lt fs_r)
+        //admit ()
+      end
+    end
+    //assume (forall p'. (theta m) h' p' ==> p' [] x);
+    //assert (lt == []);
+    //assert (fs_r == x);
+    //assume (wp2p (theta m) h' [] x)
+    //admit ()
+    end
+  | Call o args k -> admit ()
+  (*introduce forall (p':hist_post h' a). (theta m) h' p' ==> p' lt' fs_r with begin
+    introduce (theta m) h' p' ==> p' lt' fs_r with _. begin
+      
+      let p : hist_post h a = fun lt res -> p' (get_lt h h' lt) res in
+      eliminate forall p. (theta m) h p ==> p lt fs_r with p;
+      assert ((theta m) h' p');
+      assert ((theta m) h p ==> p lt fs_r);
+      admit ()
+    end
+  end*)
   
